
- $a^{m}a^{n} = a^{m+n} \rightarrow 3^{2} \cdot 3^{5}= 3^{2+5}=3^7$  
- $\frac{a^{m}}{a^{n}} = a^{m-n} \rightarrow \frac{3^{5}}{3^{2}}=3^{5-2}=3^3$ 
- $(a^{m})^{n} = a^{mn} \rightarrow (3^{2})^{5} = 3^{2 \cdot 5} = 3^{10}$ 
- $(ab)^{n}=a^{n}b^{n} \rightarrow (3\cdot 4)^{2} = 3^{2}\cdot4^{2}$ 
- $(\frac{a}{b})^{n} = \frac{a^{n}}{b^{n}} \rightarrow (\frac{3}{4})^{2} = \frac{3^{2}}{4^{2}}$ 
- $(\frac{a}{b})^{-n} = (\frac{b}{a})^{n} \rightarrow (\frac{3}{4})^{-2} = (\frac{4}{3})^{2}$
- $\frac{a^{-n}}{b^{-m}} = \frac{b^{m}}{a^{n}} \rightarrow \frac{3^{-2}}{4^{-5}} = \frac{4^{5}}{3^{2}}$ 
-









