---
tags:
  - propositional-logic
aliases: 
date: 2023-10-30
---
$p \implies q \equiv \neg p \lor q$ 
$p \implies q \equiv \neg q \implies \neg p$
$p \lor q \equiv \neg p \implies q$
$p \land q \equiv \neg(p \implies \neg q)$ 
$\neg (p \implies q) \equiv p \land \neg q$ 
$(p \implies q) \land (p \implies r) \equiv p \implies (q \land r)$     
$(p \implies r) \land (q \implies r) \equiv (p \lor q) \implies r$ 
$(p \implies q) \lor (p \implies r) \equiv p \implies (q \lor r)$ 
$(p \implies q) \land (p \implies r) \equiv p \implies (q \land r)$     
$(p \implies r) \land (q \implies r) \equiv (p \land q) \implies r$

for fucks sake.
